@prefix otgaction: <https://onthesegrounds.org/vocab/action-status#> .
@prefix dcterms: <http://purl.org/dc/terms/> .
@prefix skos: <http://www.w3.org/2004/02/skos/core#> .
@prefix rdf: <http://www.w3.org/1999/02/22-rdf-syntax-ns#> .

<https://onthesegrounds.org/vocab/action-status#> rdf:type skos:ConceptScheme;
    dcterms:title "Action Status Vocabulary"@en ;
    dcterms:description "A controlled vocabulary to describe the status of events."@en ;
    skos:hasTopConcept otgevents:actionStatus.

otgactionstatus:actionstatus rdf:type skos:Collection ;
    skos:prefLabel "Action Status"@en ;
    skos:inScheme <https://onthesegrounds.org/vocab/action-status#> ;
    skos:topConceptOf <https://onthesegrounds.org/vocab/action-status#> ;
    skos:member otgactionstatus:complete ;
    skos:member otgactionstatus:failed ;
    skos:member otgactionstatus:potential ;
    skos:member otgactionstatus:unknown .

otgactionstatus:complete rdf:type skos:Concept;
    skos:prefLabel "Complete"@en ;
    skos:definition "The action has been completed."@en ;
    skos:inScheme <https://onthesegrounds.org/vocab/action-status#>.

otgactionstatus:failed rdf:type skos:Concept;
    skos:prefLabel "Failed"@en ;
    skos:definition "The action was proposed or attempted, but was not successfully completed."@en ;
    skos:inScheme <https://onthesegrounds.org/vocab/action-status#>.

otgactionstatus:potential rdf:type skos:Concept;
    skos:prefLabel "Potential"@en ;
    skos:definition "The action has been proposed or mentioned, but has not yet taken place or been attempted."@en ;
    skos:inScheme <https://onthesegrounds.org/vocab/action-status#>.

otgactionstatus:unknown rdf:type skos:Concept;
    skos:prefLabel "Unknown"@en ;
    skos:definition "The actionâ€™s status cannot be inferred from available information."@en ;
    skos:inScheme <https://onthesegrounds.org/vocab/action-status#>.


