@prefix otgcertainty: <https://onthesegrounds.org/vocab/certainty#> .
@prefix dcterms: <http://purl.org/dc/terms/> .
@prefix skos: <http://www.w3.org/2004/02/skos/core#> .
@prefix rdf: <http://www.w3.org/1999/02/22-rdf-syntax-ns#> .

<https://onthesegrounds.org/vocab/certainty#> rdf:type skos:ConceptScheme;
    dcterms:title "Certainty Vocabulary"@en ;
    dcterms:description "A controlled vocabulary to describe the certainty of the data."@en ;
    skos:hasTopConcept otgevents:certainty.

otgcertainty:certainty rdf:type skos:Collection ;
    skos:prefLabel "Certainty"@en ;
    skos:inScheme <https://onthesegrounds.org/vocab/certainty#> ;
    skos:topConceptOf <https://onthesegrounds.org/vocab/certainty#> ;
    skos:member otgcertainty:approximate ;
    skos:member otgcertainty:inferred ;
    skos:member otgcertainty:questionable .

otgcertainty:approximate rdf:type skos:Concept;
    skos:prefLabel "Approximate"@en ;
    skos:definition "The date is not exact; the event is estimated to have taken place close to the supplied date."@en ;
    skos:inScheme <https://onthesegrounds.org/vocab/certainty#>.

otgcertainty:inferred rdf:type skos:Concept;
    skos:prefLabel "Inferred"@en ;
    skos:definition "The date of the event is not explicitly stated in the source document and has been supplied based on contextual information."@en ;
    skos:inScheme <https://onthesegrounds.org/vocab/certainty#>.

otgcertainty:questionable rdf:type skos:Concept;
    skos:prefLabel "Questionable"@en ;
    skos:definition "The date is dubious or likely to be erroneous."@en ;
    skos:inScheme <https://onthesegrounds.org/vocab/certainty#>.

