@prefix otgevents: <https://onthesegrounds.org/vocab/event-types#> .
@prefix dcterms: <http://purl.org/dc/terms/> .
@prefix skos: <http://www.w3.org/2004/02/skos/core#> .
@prefix rdf: <http://www.w3.org/1999/02/22-rdf-syntax-ns#> .

<https://onthesegrounds.org/vocab/event-types#> rdf:type skos:ConceptScheme;
    dcterms:title "Event Type Vocabulary"@en ;
    dcterms:description "A controlled vocabulary to describe the lived experiences of enslaved people who labored for colleges or universities."@en ;
    skos:hasTopConcept otgevents:eventType.

otgevents:eventType rdf:type skos:Collection ;
    skos:prefLabel "Event Type"@en ;
    skos:inScheme <https://onthesegrounds.org/vocab/event-types#> ;
    skos:topConceptOf <https://onthesegrounds.org/vocab/event-types#> ;
    skos:member otgevents:commercialTransfreedomEvents ;
    skos:member otgevents:educationEvents ;
    skos:member otgevents:freedomStatusEvents ;
    skos:member otgevents:healthEvents ;
    skos:member otgevents:laborEvents ;
    skos:member otgevents:legalEvents ;
    skos:member otgevents:lifeCourseEvents ;
    skos:member otgevents:membershipEvents ;
    skos:member otgevents:mentionEvents ;
    skos:member otgevents:narrativeEvents ;
    skos:member otgevents:provisionEvents ;
    skos:member otgevents:religionEvents ;
    skos:member otgevents:resistanceEvents ;
    skos:member otgevents:travelEvents ;
    skos:member otgevents:violenceEvents .


otgevents:commercialTransactionEvents rdf:type skos:Collection;
    skos:prefLabel "Commercial Transaction Events"@en;
    skos:inScheme <https://onthesegrounds.org/vocab/event-types#> ;
    skos:member otgevents:commercialTransaction;
    skos:member otgevents:enslavedHire;
    skos:member otgevents:enslavedLoan;
    skos:member otgevents:enslavedRental;
    skos:member otgevents:services;
    skos:member otgevents:smallGoods.

otgevents:commercialTransaction rdf:type skos:Concept;
    skos:prefLabel "Commercial Transaction"@en ;
    skos:definition "An event in which an enslaved person is part of a transaction that involves the buying or selling of goods, services, or labor"@en ;
    skos:inScheme <https://onthesegrounds.org/vocab/event-types#>.

otgevents:enslavedHire rdf:type skos:Concept;
    skos:prefLabel "Enslaved Hire"@en ;
    skos:definition "An event in which an enslaved person is hired out to an individual other than their primary enslaver for a period of time"@en ;
    skos:inScheme <https://onthesegrounds.org/vocab/event-types#> .

otgevents:enslavedLoan rdf:type skos:Concept;
    skos:prefLabel "Enslaved Loan"@en ;
    skos:definition "An event in which an enslaved person is loaned to an individual other than their primary enslaver for a period of time"@en ;
    skos:inScheme <https://onthesegrounds.org/vocab/event-types#> .

otgevents:services rdf:type skos:Concept;
    skos:prefLabel "Services"@en ;
    skos:definition "An event in which an enslaved person is buying or selling of services (laundry, mending, blacksmithing, midwifery)"@en ;
    skos:inScheme <https://onthesegrounds.org/vocab/event-types#> .

otgevents:smallGoods rdf:type skos:Concept;
    skos:prefLabel "Small Goods"@en ;
    skos:definition "An event in which an enslaved person is buying or selling small goods (crafts, foodstuffs, etc.)"@en ;
    skos:inScheme <https://onthesegrounds.org/vocab/event-types#> .


otgevents:educationEvents rdf:type skos:Collection;
    skos:prefLabel "Education Events"@en;
    skos:inScheme <https://onthesegrounds.org/vocab/event-types#> ;
    skos:member otgevents:education.
    skos:member otgevents:teaching

otgevents:education rdf:type skos:Concept;
    skos:prefLabel "Education"@en ;
    skos:definition "An event in which an enslaved person is being educated"@en ;
    skos:inScheme <https://onthesegrounds.org/vocab/event-types#> .

otgevents:education rdf:type skos:Concept;
    skos:prefLabel "Teaching"@en ;
    skos:definition "An event in which an enslaved person is teaching someone else"@en ;
    skos:inScheme <https://onthesegrounds.org/vocab/event-types#> .


otgevents:freedomStatusEvents rdf:type skos:Collection;
    skos:prefLabel "Freedom Status Events"@en;
    skos:inScheme <https://onthesegrounds.org/vocab/event-types#> ;
    skos:member otgevents:freedomStatus;
    skos:member otgevents:dispute;
    skos:member otgevents:emancipation;
    skos:member otgevents:enslavement;
    skos:member otgevents:exchange;
    skos:member otgevents:manumission;
    skos:member otgevents:purchase;
    skos:member otgevents:sale;
    skos:member otgevents:transfer.

otgevents:freedomStatus rdf:type skos:Concept;
    skos:prefLabel "Freedom Status"@en ;
    skos:definition "An event in which an enslaved person is part of a transaction that changes their status or ownership"@en ;
    skos:inScheme <https://onthesegrounds.org/vocab/event-types#>.

otgevents:dispute rdf:type skos:Concept;
    skos:prefLabel "Dispute"@en ;
    skos:definition "An event in which there is a dispute over an enslaved person’s freedom status"@en ;
    skos:inScheme <https://onthesegrounds.org/vocab/event-types#>.

otgevents:enslavement rdf:type skos:Concept;
    skos:prefLabel "Emancipationt"@en ;
    skos:definition "An event in which an enslaved person is freed by an order of a state"@en ;
    skos:inScheme <https://onthesegrounds.org/vocab/event-types#>.

otgevents:enslavement rdf:type skos:Concept;
    skos:prefLabel "Enslavement"@en ;
    skos:definition "An event in which a person’s status changes from free to enslaved"@en ;
    skos:inScheme <https://onthesegrounds.org/vocab/event-types#>.

otgevents:exchange rdf:type skos:Concept;
    skos:prefLabel "Exchange"@en ;
    skos:definition "An event in which an enslaved person is exchanged for another enslaved person or goods by a free person who has control over them"@en ;
    skos:inScheme <https://onthesegrounds.org/vocab/event-types#>.

otgevents:manumission rdf:type skos:Concept;
    skos:prefLabel "Manumission"@en ;
    skos:definition "An event in which an enslaved person is freed by an owner(s)"@en ;
    skos:inScheme <https://onthesegrounds.org/vocab/event-types#>.

otgevents:purchase rdf:type skos:Concept;
    skos:prefLabel "Purchase"@en ;
    skos:definition "An event in which an enslaved person is purchased by a free person or an organization"@en ;
    skos:inScheme <https://onthesegrounds.org/vocab/event-types#>.

otgevents:sale rdf:type skos:Concept;
    skos:prefLabel "Sale"@en ;
    skos:definition "An event in which an enslaved person is sold by their owner(s)"@en ;
    skos:inScheme <https://onthesegrounds.org/vocab/event-types#>.

otgevents:transfer rdf:type skos:Concept;
    skos:prefLabel "Transfer"@en ;
    skos:definition "An event in which ownership or control of an enslaved person is transferred from one entity to another"@en ;
    skos:inScheme <https://onthesegrounds.org/vocab/event-types#>.


otgevents:healthEvents rdf:type skos:Collection;
    skos:prefLabel "Health Events"@en;
    skos:inScheme <https://onthesegrounds.org/vocab/event-types#> ;
    skos:member otgevents:health;
    skos:member otgevents:childbirth;
    skos:member otgevents:illness;
    skos:member otgevents:injury;
    skos:member otgevents:medicalTreatment;
    skos:member otgevents:pregnancy.

otgevents:health rdf:type skos:Concept;
    skos:prefLabel "Health"@en ;
    skos:definition "An event in which an enslaved person is ill or undergoes a major bodily issue, sometimes requiring attendance from a healthcare provider"@en ;
    skos:inScheme <https://onthesegrounds.org/vocab/event-types#>.

otgevents:childbirth rdf:type skos:Concept;
    skos:prefLabel "Childbirth"@en ;
    skos:definition "An event in which a woman gives birth to a child"@en ;
    skos:inScheme <https://onthesegrounds.org/vocab/event-types#>.

otgevents:illness rdf:type skos:Concept;
    skos:prefLabel "Illness"@en ;
    skos:definition "An event in which an enslaved person experiences sickness or disease"@en ;
    skos:inScheme <https://onthesegrounds.org/vocab/event-types#>.

otgevents:injury rdf:type skos:Concept;
    skos:prefLabel "Injury"@en ;
    skos:definition "An event in which an enslaved person experiences a physical trauma to the body through accident, assault, or other causes"@en ;
    skos:inScheme <https://onthesegrounds.org/vocab/event-types#>.

otgevents:medicalTreatment rdf:type skos:Concept;
    skos:prefLabel "Medical Treatment"@en ;
    skos:definition "An event in which an enslaved person receives treatment for illness, injury, or other medical conditions"@en ;
    skos:inScheme <https://onthesegrounds.org/vocab/event-types#>.

otgevents:pregnancy rdf:type skos:Concept;
    skos:prefLabel "Pregnancy"@en ;
    skos:definition "An event in which an enslaved person is pregnant"@en ;
    skos:inScheme <https://onthesegrounds.org/vocab/event-types#>.


otgevents:laborEvents rdf:type skos:Collection;
    skos:prefLabel "Labor Events"@en;
    skos:inScheme <https://onthesegrounds.org/vocab/event-types#> ;
    skos:member otgevents:labor;
    skos:member otgevents:agriculture;
    skos:member otgevents:domestic;
    skos:member otgevents:midwifery;
    skos:member otgevents:skilled.

otgevents:labor rdf:type skos:Concept;
    skos:prefLabel "Labor"@en ;
    skos:definition "An event in which an enslaved person is performing some kind of work"@en ;
    skos:inScheme <https://onthesegrounds.org/vocab/event-types#>.

otgevents:agriculture rdf:type skos:Concept;
    skos:prefLabel "Agriculture"@en ;
    skos:definition "An event in which a person works to raise a crop or livestock"@en ;
    skos:inScheme <https://onthesegrounds.org/vocab/event-types#>.

otgevents:domestic rdf:type skos:Concept;
    skos:prefLabel "Domestic"@en ;
    skos:definition "An event in which a person works at the tasks required to keep a home, e.g. cooking, cleaning, laundry"@en ;
    skos:inScheme <https://onthesegrounds.org/vocab/event-types#>.

otgevents:midwifery rdf:type skos:Concept;
    skos:prefLabel "Midwifery"@en ;
    skos:definition "An event in which a person assists with the birthing of a child"@en ;
    skos:inScheme <https://onthesegrounds.org/vocab/event-types#>.

otgevents:skilled rdf:type skos:Concept;
    skos:prefLabel "Skilled"@en ;
    skos:definition "An event in which a person participates in labor that requires specialized knowledge and experience, e.g. carpentry, blacksmithing, tailoring, shoemaking"@en ;
    skos:inScheme <https://onthesegrounds.org/vocab/event-types#>.


otgevents:legalEvents rdf:type skos:Collection;
    skos:prefLabel "Legal Events"@en;
    skos:inScheme <https://onthesegrounds.org/vocab/event-types#> ;
    skos:member otgevents:legal;
    skos:member otgevents:civilCase;
    skos:member otgevents:criminalCase;
    skos:member otgevents:dowry;
    skos:member otgevents:freedomPetition;
    skos:member otgevents:manumissionFiling;
    skos:member otgevents:probate;
    skos:member otgevents:taxFiling;
    skos:member otgevents:will.

otgevents:legal rdf:type skos:Concept;
    skos:prefLabel "Legal"@en ;
    skos:definition "An event that involves a legal filing or proceeding related to an enslaved person"@en ;
    skos:inScheme <https://onthesegrounds.org/vocab/event-types#>.

otgevents:civilCase rdf:type skos:Concept;
    skos:prefLabel "Civil case"@en ;
    skos:definition "A court proceeding involving an enslaved person based on a non-criminal issue"@en ;
    skos:inScheme <https://onthesegrounds.org/vocab/event-types#>.

otgevents:criminalCase rdf:type skos:Concept;
    skos:prefLabel "Criminal case"@en ;
    skos:definition "A court proceeding involving an enslaved person that relates to a criminal statute"@en ;
    skos:inScheme <https://onthesegrounds.org/vocab/event-types#>.

otgevents:dowry rdf:type skos:Concept;
    skos:prefLabel "Dowry"@en ;
    skos:definition "A legal filing involving an enslaved person related to the transfer of property on the occasion of a marriage"@en ;
    skos:inScheme <https://onthesegrounds.org/vocab/event-types#>.

otgevents:freedomPetition rdf:type skos:Concept;
    skos:prefLabel "Freedom petition"@en ;
    skos:definition "A legal petition from an enslaved person claiming their freedom rights"@en ;
    skos:inScheme <https://onthesegrounds.org/vocab/event-types#>.

otgevents:manumissionFiling rdf:type skos:Concept;
    skos:prefLabel "Manumission filing"@en ;
    skos:definition "A legal filing that registers the freeing of an enslaved person"@en ;
    skos:inScheme <https://onthesegrounds.org/vocab/event-types#>.

otgevents:probate rdf:type skos:Concept;
    skos:prefLabel "Probate"@en ;
    skos:definition "A legal filing that provides an accounting of a person’s estate after their death"@en ;
    skos:inScheme <https://onthesegrounds.org/vocab/event-types#>.

otgevents:taxFiling rdf:type skos:Concept;
    skos:prefLabel "Tax filing"@en ;
    skos:definition "A legal filing that provides an accounting of property for the purposes of taxation or dispute about taxation"@en ;
    skos:inScheme <https://onthesegrounds.org/vocab/event-types#>.

otgevents:will rdf:type skos:Concept;
    skos:prefLabel "Will"@en ;
    skos:definition "A legal filing outlining a person’s wishes for the disposition of their property upon their death"@en ;
    skos:inScheme <https://onthesegrounds.org/vocab/event-types#>.


otgevents:lifeCourseEvents rdf:type skos:Collection;
    skos:prefLabel "Life Course Events"@en;
    skos:inScheme <https://onthesegrounds.org/vocab/event-types#> ;
    skos:member otgevents:lifeCourse;
    skos:member otgevents:birth;
    skos:member otgevents:burial;
    skos:member otgevents:death;
    skos:member otgevents:marriage.

otgevents:lifeCourse rdf:type skos:Concept;
    skos:prefLabel "Life course"@en ;
    skos:definition "An event involving an enslaved person that is part of the normal course of a human lifetime"@en ;
    skos:inScheme <https://onthesegrounds.org/vocab/event-types#>.

otgevents:birth rdf:type skos:Concept;
    skos:prefLabel "Birth"@en ;
    skos:definition "An event in which a person is born "@en ;
    skos:inScheme <https://onthesegrounds.org/vocab/event-types#>.

otgevents:burial rdf:type skos:Concept;
    skos:prefLabel "Burial"@en ;
    skos:definition "An event in which an enslaved person is interred"@en ;
    skos:inScheme <https://onthesegrounds.org/vocab/event-types#>.

otgevents:death rdf:type skos:Concept;
    skos:prefLabel "Death"@en ;
    skos:definition "An event in which an enslaved person dies"@en ;
    skos:inScheme <https://onthesegrounds.org/vocab/event-types#>.

otgevents:marriage rdf:type skos:Concept;
    skos:prefLabel "Marriage"@en ;
    skos:definition "An event in which an enslaved person participates in a ritual to mark their commitment to a long term relationship with another person"@en ;
    skos:inScheme <https://onthesegrounds.org/vocab/event-types#>.


otgevents:membershipEvents rdf:type skos:Collection;
    skos:prefLabel "Membership or Participation Events"@en;
    skos:inScheme <https://onthesegrounds.org/vocab/event-types#> ;
    skos:member otgevents:membership;
    skos:member otgevents:fraternalOrganization;
    skos:member otgevents:military.

otgevents:membership rdf:type skos:Concept;
    skos:prefLabel "Membership"@en ;
    skos:definition "An event in which an enslaved person joins or participates in a group"@en ;
    skos:inScheme <https://onthesegrounds.org/vocab/event-types#>.

otgevents:fraternalOrganization rdf:type skos:Concept;
    skos:prefLabel "Fraternal organization"@en ;
    skos:definition "An event in which an enslaved person joins a cooperative organization of peers"@en ;
    skos:inScheme <https://onthesegrounds.org/vocab/event-types#>.

otgevents:military rdf:type skos:Concept;
    skos:prefLabel "Military"@en ;
    skos:definition "An event in which an enslaved person joins a segment of armed forces"@en ;
    skos:inScheme <https://onthesegrounds.org/vocab/event-types#>.


otgevents:mentionEvents rdf:type skos:Collection;
    skos:prefLabel "Mention Events"@en;
    skos:inScheme <https://onthesegrounds.org/vocab/event-types#> ;
    skos:member otgevents:mention.
    skos:member otgevents:disappearance.
    skos:member otgevents:inventory.

otgevents:mention rdf:type skos:Concept;
    skos:prefLabel "Mention"@en ;
    skos:definition "An event in which an enslaved person is noted in an unspecified way, e.g. correspondence that notes an encounter"@en ;
    skos:inScheme <https://onthesegrounds.org/vocab/event-types#>.

otgevents:disappearance rdf:type skos:Concept;
    skos:prefLabel "Disappearance"@en ;
    skos:definition "An event in which an enslaved person is missing for an indeterminate reason"@en ;
    skos:inScheme <https://onthesegrounds.org/vocab/event-types#>.

otgevents:inventory rdf:type skos:Concept;
    skos:prefLabel "Inventory"@en ;
    skos:definition "An event in which an enslaved person is recorded in a list of enslaved people or other property (excluding legal documents)"@en ;
    skos:inScheme <https://onthesegrounds.org/vocab/event-types#>.


otgevents:narrativeEvents rdf:type skos:Collection;
    skos:prefLabel "Narrative Events"@en;
    skos:inScheme <https://onthesegrounds.org/vocab/event-types#> ;
    skos:member otgevents:narrative;
    skos:member otgevents:autobiography;
    skos:member otgevents:testimony.

otgevents:narrative rdf:type skos:Concept;
    skos:prefLabel "Narrative"@en ;
    skos:definition "An event in which an enslaved person tells their own story"@en ;
    skos:inScheme <https://onthesegrounds.org/vocab/event-types#>.

otgevents:autobiography rdf:type skos:Concept;
    skos:prefLabel "Autobiography"@en ;
    skos:definition "An instance in which an enslaved person relates or writes their life story"@en ;
    skos:inScheme <https://onthesegrounds.org/vocab/event-types#>.

otgevents:testimony rdf:type skos:Concept;
    skos:prefLabel "Testimony"@en ;
    skos:definition "An instance in which an enslaved person relates or writes an account of an event or circumstances"@en ;
    skos:inScheme <https://onthesegrounds.org/vocab/event-types#>.


otgevents:provisionEvents rdf:type skos:Collection;
    skos:prefLabel "Provision Events"@en;
    skos:inScheme <https://onthesegrounds.org/vocab/event-types#> ;
    skos:member otgevents:provision;
    skos:member otgevents:clothing;
    skos:member otgevents:food;
    skos:member otgevents:housing;
    skos:member otgevents:supplies.

otgevents:provision rdf:type skos:Concept;
    skos:prefLabel "Provision"@en ;
    skos:definition "An event in which provisions are acquired for use by enslaved people"@en ;
    skos:inScheme <https://onthesegrounds.org/vocab/event-types#>.

otgevents:clothing rdf:type skos:Concept;
    skos:prefLabel "Clothing"@en ;
    skos:definition "An event in which clothing for an enslaved person is purchased, is bartered for, or is made"@en ;
    skos:inScheme <https://onthesegrounds.org/vocab/event-types#>.

otgevents:food rdf:type skos:Concept;
    skos:prefLabel "Food"@en ;
    skos:definition "An event in which clothing for an enslaved person is purchased, is bartered for, or is prepared"@en ;
    skos:inScheme <https://onthesegrounds.org/vocab/event-types#>.

otgevents:housing rdf:type skos:Concept;
    skos:prefLabel "Housing"@en ;
    skos:definition "An event in which clothing for an enslaved person is purchased, is bartered for, or is made"@en ;
    skos:inScheme <https://onthesegrounds.org/vocab/event-types#>.

otgevents:supplies rdf:type skos:Concept;
    skos:prefLabel "Supplies"@en ;
    skos:definition "An event in which clothing for an enslaved person is purchased, is bartered for, or is made"@en ;
    skos:inScheme <https://onthesegrounds.org/vocab/event-types#>.


otgevents:religionEvents rdf:type skos:Collection;
    skos:prefLabel "Religious Events"@en;
    skos:inScheme <https://onthesegrounds.org/vocab/event-types#> ;
    skos:member otgevents:religious;
    skos:member otgevents:baptism;
    skos:member otgevents:communion;
    skos:member otgevents:confession;
    skos:member otgevents:lastRites;
    skos:member otgevents:marriageSacrament;
    skos:member otgevents:music;
    skos:member otgevents:ordination;
    skos:member otgevents:preaching.

otgevents:religious rdf:type skos:Concept;
    skos:prefLabel "Religious"@en ;
    skos:definition "An event in which an enslaved person participates that is religious in nature, sometimes involving the presence of a member of the clergy"@en ;
    skos:inScheme <https://onthesegrounds.org/vocab/event-types#>.

otgevents:baptism rdf:type skos:Concept;
    skos:prefLabel "Baptism"@en ;
    skos:definition "An event in which an enslaved person is initiated into a Christian denomination"@en ;
    skos:inScheme <https://onthesegrounds.org/vocab/event-types#>.

otgevents:communion rdf:type skos:Concept;
    skos:prefLabel "Communion"@en ;
    skos:definition "An event in which a person participates in the reception of the Eucharist"@en ;
    skos:inScheme <https://onthesegrounds.org/vocab/event-types#>.

otgevents:confession rdf:type skos:Concept;
    skos:prefLabel "Confession"@en ;
    skos:definition "An event in which a person confesses their sins to a priest and seeks absolution"@en ;
    skos:inScheme <https://onthesegrounds.org/vocab/event-types#>.

otgevents:lastRites rdf:type skos:Concept;
    skos:prefLabel "Last rites"@en ;
    skos:definition "An event in which a member of the clergy offers a blessing sacrament and final absolution for individuals on the verge of death"@en ;
    skos:inScheme <https://onthesegrounds.org/vocab/event-types#>.

otgevents:marriageSacrament rdf:type skos:Concept;
    skos:prefLabel "Marriage sacrament"@en ;
    skos:definition "An event in which two people are bound in matrimony that is officiated by a member of the clergy"@en ;
    skos:inScheme <https://onthesegrounds.org/vocab/event-types#>.

otgevents:music rdf:type skos:Concept;
    skos:prefLabel "Music"@en ;
    skos:definition "An event in which a person sings or plays an instrument as a form of worship or religious praise"@en ;
    skos:inScheme <https://onthesegrounds.org/vocab/event-types#>.

otgevents:ordination rdf:type skos:Concept;
    skos:prefLabel "Ordination"@en ;
    skos:definition "An event in which a bishop ordains a person into the priesthood or ministry"@en ;
    skos:inScheme <https://onthesegrounds.org/vocab/event-types#>.

otgevents:preaching rdf:type skos:Concept;
    skos:prefLabel "Preaching"@en ;
    skos:definition "An event in which a person delivers a sermon or a homily in the context of religious worship"@en ;
    skos:inScheme <https://onthesegrounds.org/vocab/event-types#>.

#
# Do we need Mass? or services?
# 

otgevents:resistanceEvents rdf:type skos:Collection;
    skos:prefLabel "Resistance Events"@en;
    skos:inScheme <https://onthesegrounds.org/vocab/event-types#> ;
    skos:member otgevents:resistance;
    skos:member otgevents:appeal;
    skos:member otgevents:defense;
    skos:member otgevents:freedomSeeking;
    skos:member otgevents:propertyDestruction;
    skos:member otgevents:workSlowdown.

otgevents:resistance rdf:type skos:Concept;
    skos:prefLabel "Resistance"@en ;
    skos:definition "An event in which an enslaved person takes action to resist their status or treatment, or that of a compatriot"@en ;
    skos:inScheme <https://onthesegrounds.org/vocab/event-types#>.

otgevents:appeal rdf:type skos:Concept;
    skos:prefLabel "Appeal"@en ;
    skos:definition "A written or oral request for change in treatment or circumstances"@en ;
    skos:inScheme <https://onthesegrounds.org/vocab/event-types#>.

otgevents:defense rdf:type skos:Concept;
    skos:prefLabel "Defense"@en ;
    skos:definition "An event in which one person comes to the defense of self or another person"@en ;
    skos:inScheme <https://onthesegrounds.org/vocab/event-types#>.

otgevents:freedomSeeking rdf:type skos:Concept;
    skos:prefLabel "Freedom seeking"@en ;
    skos:definition "An event in which an enslaved person leaves the controlling jurisdiction of their owner permanently or for a time"@en ;
    skos:inScheme <https://onthesegrounds.org/vocab/event-types#>.

otgevents:propertyDestruction rdf:type skos:Concept;
    skos:prefLabel "Property destruction"@en ;
    skos:definition "An event in which someone purposefully damages someone else’s property"@en ;
    skos:inScheme <https://onthesegrounds.org/vocab/event-types#>.

otgevents:workSlowdown rdf:type skos:Concept;
    skos:prefLabel "Work slowdown or stoppage"@en ;
    skos:definition "An event in which an enslaved person performs work slowly or not at all"@en ;
    skos:inScheme <https://onthesegrounds.org/vocab/event-types#>.


otgevents:travelEvents rdf:type skos:Collection;
    skos:prefLabel "Travel Events"@en;
    skos:inScheme <https://onthesegrounds.org/vocab/event-types#> ;
    skos:member otgevents:travel;
    skos:member otgevents:importation;
    skos:member otgevents:relocation;
    skos:member otgevents:temporary.

otgevents:travel rdf:type skos:Concept;
    skos:prefLabel "Travel"@en ;
    skos:definition "An event in which an enslaved person moves from one location to another, often at the behest of an owner or trader"@en ;
    skos:inScheme <https://onthesegrounds.org/vocab/event-types#>.

otgevents:importation rdf:type skos:Concept;
    skos:prefLabel "Importation"@en ;
    skos:definition "An event in which an enslaved person of African descent is brought to the Americas, e.g. a transatlantic voyage from an African port to the Chesapeake region via ship"@en ;
    skos:inScheme <https://onthesegrounds.org/vocab/event-types#>.

otgevents:relocation rdf:type skos:Concept;
    skos:prefLabel "Relocation"@en ;
    skos:definition "An event in which an enslaved person is transferred from one primary residence to another"@en ;
    skos:inScheme <https://onthesegrounds.org/vocab/event-types#>.

otgevents:temporary rdf:type skos:Concept;
    skos:prefLabel "Temporary"@en ;
    skos:definition "An event in which an enslaved person moves from one location to another for a finite period of time, e.g. the transfer of someone from one farm to another for a work assignment, or the granting of a travel pass for a person to visit family"@en ;
    skos:inScheme <https://onthesegrounds.org/vocab/event-types#>.


otgevents:violenceEvents rdf:type skos:Collection;
    skos:prefLabel "Violence Events"@en;
    skos:inScheme <https://onthesegrounds.org/vocab/event-types#> ;
    skos:member otgevents:violence;
    skos:member otgevents:capture;
    skos:member otgevents:harassment;
    skos:member otgevents:jailing;
    skos:member otgevents:physicalAssault;
    skos:member otgevents:postmortemAbuse;
    skos:member otgevents:punishment;
    skos:member otgevents:sexualAssault.

otgevents:violence rdf:type skos:Concept;
    skos:prefLabel "Violence"@en ;
    skos:definition "An event in which an enslaved person is involved in a violent altercation, often at the hands of another, frequently a non-enslaved person"@en ;
    skos:inScheme <https://onthesegrounds.org/vocab/event-types#>.

otgevents:capture rdf:type skos:Concept;
    skos:prefLabel "Capture"@en ;
    skos:definition "An event in which an enslaved person is apprehended by some external entity, such as a slave patrol"@en ;
    skos:inScheme <https://onthesegrounds.org/vocab/event-types#>.

otgevents:harassment rdf:type skos:Concept;
    skos:prefLabel "Harassment"@en ;
    skos:definition "An event in which a an enslaved person is subjected to verbal taunting or abuse"@en ;
    skos:inScheme <https://onthesegrounds.org/vocab/event-types#>.

otgevents:jailing rdf:type skos:Concept;
    skos:prefLabel "Jailing"@en ;
    skos:definition "An event in which an enslaved person is confined by the state or a municipal authority for some wrongdoing or transgression"@en ;
    skos:inScheme <https://onthesegrounds.org/vocab/event-types#>.

otgevents:jailing rdf:type skos:Concept;
    skos:prefLabel "Perpetrating"@en ;
    skos:definition "An event in which an enslaved person performs a violent act"@en ;
    skos:inScheme <https://onthesegrounds.org/vocab/event-types#>.

otgevents:physicalAssault rdf:type skos:Concept;
    skos:prefLabel "Physical assault"@en ;
    skos:definition "An event in which an enslaved person is physically harmed by another person, excluding sexual violence"@en ;
    skos:inScheme <https://onthesegrounds.org/vocab/event-types#>.

otgevents:postmortemAbuse rdf:type skos:Concept;
    skos:prefLabel "Postmortem abuse"@en ;
    skos:definition "An event in which the body of a deceased enslaved person is used in ways to which they did not consent, e.g. medical or scientific research, etc."@en ;
    skos:inScheme <https://onthesegrounds.org/vocab/event-types#>.

otgevents:punishment rdf:type skos:Concept;
    skos:prefLabel "Punishment"@en ;
    skos:definition "An event in which an enslaved person is punished in a way that does not include physical assault, such as increased labor, withholding of provisions"@en ;
    skos:inScheme <https://onthesegrounds.org/vocab/event-types#>.

otgevents:sexualAssault rdf:type skos:Concept;
    skos:prefLabel "Sexual Assault"@en ;
    skos:definition "An event in which a person subjects an enslaved person to harm that is of a sexual nature, eg. unwanted touching, rape, etc."@en ;
    skos:inScheme <https://onthesegrounds.org/vocab/event-types#>.
