@prefix otgfreedomstatus: <https://onthesegrounds.org/vocab/freedom-status#> .
@prefix dcterms: <http://purl.org/dc/terms/> .
@prefix skos: <http://www.w3.org/2004/02/skos/core#> .
@prefix rdf: <http://www.w3.org/1999/02/22-rdf-syntax-ns#> .

<https://onthesegrounds.org/vocab/freedom-status#> rdf:type skos:ConceptScheme;
    dcterms:title "Freedom Status Vocabulary"@en ;
    dcterms:description "A controlled vocabulary to indicate the state of freedom or enslavement of the primary participant that the time of the event."@en ;
    skos:hasTopConcept otgevents:freedomStatus.

otgfreedomstatus:freedomStatus rdf:type skos:Collection ;
    skos:prefLabel "Freedom Status"@en ;
    skos:inScheme <https://onthesegrounds.org/vocab/freedom-status#> ;
    skos:topConceptOf <https://onthesegrounds.org/vocab/freedom-status#> ;
    skos:member otgfreedomstatus:enslaved ;
    skos:member otgfreedomstatus:free ;
    skos:member otgfreedomstatus:transition ;
    skos:member otgfreedomstatus:unknown .
    

otgfreedomstatus:enslaved rdf:type skos:Concept;
    skos:prefLabel "Enslaved"@en ;
    skos:definition "A condition of perpetual hereditary unfreedom that is central to the system of forced labor"@en ;
    skos:inScheme <https://onthesegrounds.org/vocab/freedom-status#>.

otgfreedomstatus:free rdf:type skos:Concept;
    skos:prefLabel "Free"@en ;
    skos:definition "A condition of autonomy and self possession that allows a person to control their own labor, movement, and social engagement"@en ;
    skos:inScheme <https://onthesegrounds.org/vocab/freedom-status#>.

otgfreedomstatus:transition rdf:type skos:Concept;
    skos:prefLabel "Transition"@en ;
    skos:definition "A condition of freedom that is in transition from enslaved to free or free to enslaved"@en ;
    skos:inScheme <https://onthesegrounds.org/vocab/freedom-status#>.

otgfreedomstatus:unknown rdf:type skos:Concept;
    skos:prefLabel "Unknown"@en ;
    skos:definition "A condition in which a personâ€™s status as enslaved or free cannot be inferred from the available information"@en ;
    skos:inScheme <https://onthesegrounds.org/vocab/freedom-status#>.


